updates

Veritas.Verifier.EAC.fst
@@ -838,7 +838,6 @@ let lemma_non_eac_evicted_merkle_addm (#p:pos)
       (* which gives us a hash collision *)
       SingleHashCollision (Collision v v_e)     
     )
-*)
 
 let lemma_non_eac_evicted_blum_addm (#p:pos)   
   (itsl: non_eac_ts_log p{
@@ -886,10 +885,8 @@ let lemma_non_eac_evicted_blum_addm (#p:pos)
       lemma_proving_ancestor_blum_bit itsli k;
       hash_collision_contra()      
   )
+*)
 
-(******************************************)
-
-(*
 let lemma_non_eac_evicted_merkle_addb (#p:pos)   
   (itsl: non_eac_ts_log p{
     g_hash_verifiable (partition_idx_seq itsl) /\  
@@ -917,20 +914,20 @@ let lemma_non_eac_evicted_merkle_addb (#p:pos)
       let vsi = verifier_thread_state itsli tid in
 
       let itsli' = its_prefix itsl (i + 1) in
-      let vsi' = verifier_thread_state itsli tid in    
+      let vsi' = verifier_thread_state itsli' tid in    
       lemma_verifier_thread_state_extend itsli';  
       assert(vsi' == t_verify_step vsi e);    
-
 
       (* number of blum evicts is the same as blum adds in the first i entries *)
       lemma_evict_add_count_same_evictedm itsli k;
       assert(MS.size (ts_add_set_key itsli k) = MS.size (ts_evict_set_key itsli k));
-    
+
       (* the ith element is a blum add *)
       assert(is_blum_add #p (e,tid));
-      lemma_ts_add_set_key_extend itsli;
-      assert(ts_add_set_key itsli' k == ts_add_set_key itsli k);
-      
+      lemma_ts_add_set_key_extend itsli';
+      assert(ts_add_set_key itsli' k == add_elem (ts_add_set_key itsli k)
+                                                 (blum_add_elem #p (e,tid)));
+
       (* the ith element is not a blum evict *)
       assert(not (is_blum_evict (index itsl i)));
       lemma_ts_evict_set_key_extend2 itsli';
@@ -943,36 +940,47 @@ let lemma_non_eac_evicted_merkle_addb (#p:pos)
       (* this implies that in the first (i+1) entries there is an element whose membership in 
          * add multiset is > its membership in evict multiset *)
       let be = diff_elem (ts_add_set_key itsli' k) (ts_evict_set_key itsli' k) in
+      lemma_ts_add_set_key_contains_only itsli' k be;
+      assert(MH.key_of be = k);
+
       lemma_mem_key_add_set_same itsli' be;
       lemma_mem_key_evict_set_same itsli' be;  
       assert(MS.mem be (ts_add_set itsli') > MS.mem be (ts_evict_set itsli'));
 
-      (* this implies that in the first (i+1) entries there is an element whose membership in 
-         * add multiset is > its membership in evict multiset *)
-      let be = diff_elem (ts_add_set_key itsli' k) (ts_evict_set_key itsli' k) in
-      lemma_mem_key_add_set_same itsli' be;
-      lemma_mem_key_evict_set_same itsli' be;  
-      assert(MS.mem be (ts_add_set itsli') > MS.mem be (ts_evict_set itsli'));
-
+      (* the index of be in the add set *)
+      let i_be = some_add_elem_idx itsli' be in
+      assert(i_be <= i);
 
       (* from clock orderedness any evict_set entry for be should happen before i *)
-      lemma_evict_before_add2 itsl i;
-      assert(MS.mem be (ts_evict_set itsl) = MS.mem be (ts_evict_set itsli'));
-      assert(MS.mem be (ts_add_set itsli') > MS.mem be (ts_evict_set itsl));
+      lemma_evict_before_add2 itsl i_be;
+      assert(MS.mem be (ts_evict_set itsl) = MS.mem be (ts_evict_set (its_prefix itsl i_be)));
 
+      (* any set membership is monotonic *)
       lemma_mem_monotonic be itsl (i + 1);
+      lemma_mem_monotonic be itsli' i_be;
+      assert(MS.mem be (ts_add_set itsl) >= MS.mem be (ts_add_set itsli'));
+      assert(MS.mem be (ts_evict_set itsl) = MS.mem be (ts_evict_set itsli'));
+
+      (* this implies the membership of be in (overall) addset > membership in evict set *)
+      (* so these two sets are not equal providing a hash collision *)
       assert(MS.mem be (ts_add_set itsl) > MS.mem be (ts_evict_set itsl));  
 
       MS.lemma_not_equal (ts_add_set itsl) (ts_evict_set itsl) be;
-      assert(~ (g_add_set gl == g_evict_set gl));
+      assert(~( (ts_add_set itsl) == (ts_evict_set itsl)));
 
+      lemma_ts_add_set_correct itsl;
+      lemma_ts_evict_set_correct itsl;
+      assert(~ (g_add_set gl == g_evict_set gl));
 
       lemma_g_hadd_correct gl;
       lemma_ghevict_correct gl;
 
-      MultiHashCollision (MSCollision (g_add_seq gl) (g_evict_seq gl))      
+      MultiHashCollision (MSCollision (g_add_seq gl) (g_evict_seq gl))
   )
 
+(******************************************)
+
+(*
 let lemma_non_eac_evicted_blum_addb (#p:pos)   
   (itsl: non_eac_ts_log p{
     g_hash_verifiable (partition_idx_seq itsl) /\  
